src/FiniteSetADTs/FiniteSetADT.v
@@ -1,0 +1,106 @@
+(** * Definition of the finite set spec *)
+Require Import Coq.Strings.String Coq.Sets.Ensembles Coq.Sets.Finite_sets Coq.Lists.List Permutation.
+Require Import ADT ADT.ComputationalADT ADTRefinement.Core ADTNotation ADTRefinement.GeneralRefinements Common.AdditionalEnsembleDefinitions Common.AdditionalEnsembleLemmas.
+
+Set Implicit Arguments.
+
+Local Open Scope string_scope.
+
+(** TODO: Figure out where Facade words live, and use that *)
+Module Type BedrockWordT.
+  Axiom W : Type.
+  Axiom wzero : W.
+  Axiom wplus : W -> W -> W.
+End BedrockWordT.
+
+Module Export BedrockWord : BedrockWordT.
+  Definition W := nat.
+  Definition wzero := 0.
+  Definition wplus := plus.
+End BedrockWord.
+
+(** TODO: Test: Do we get a speedup if we replace these definitions
+    with [{| bindex := "$STRING-HERE" |}]? *)
+Definition sEmpty := "Empty".
+Definition sAdd := "Add".
+Definition sRemove := "Remove".
+Definition sIn := "In".
+Definition sSize := "Size".
+
+(** We define the interface for finite sets *)
+(** QUESTION: Does Facade give us any other methods?  Do we want to
+    provide any other methods? *)
+Definition FiniteSetSig : ADTSig :=
+  ADTsignature {
+      Constructor sEmpty : unit -> rep,
+      Method sAdd : rep x W -> rep x unit,
+      Method sRemove : rep x W -> rep x unit,
+      Method sIn : rep x W -> rep x bool,
+      Method sSize : rep x unit -> rep x nat
+    }.
+
+(** And now the spec *)
+Definition FiniteSetSpec : ADT FiniteSetSig :=
+  ADTRep (Ensemble W) {
+    Def Constructor sEmpty (_ : unit) : rep := ret (Empty_set _),
+
+    Def Method sAdd (xs : rep , x : W) : unit :=
+      ret (Add _ xs x, tt),
+
+    Def Method sRemove (xs : rep , x : W) : unit :=
+      ret (Subtract _ xs x, tt),
+
+    Def Method sIn (xs : rep , x : W) : bool :=
+        (b <- { b : bool | b = true <-> Ensembles.In _ xs x };
+         ret (xs, b)),
+
+    Def Method sSize (xs : rep , _ : unit) : nat :=
+          (n <- { n : nat | cardinal _ xs n };
+           ret (xs, n))
+  }.
+
+
+(** Now we spec out two examples, the count of the unique elements in
+    a list, and the sum of the unique elements in a list. *)
+
+Definition elements {A} (ls : list A) : Ensemble A := fun x => List.In x ls.
+
+Definition cardinal {A} (ls : list A) : Comp nat
+  := Pick (cardinal _ (elements ls)).
+
+Definition to_list {A} (S : Ensemble A) : Comp (list A) :=
+  { ls : list _ | EnsembleListEquivalence S ls }.
+
+(** QUESTION: Should I switch [fold_right] and [Ensemble_fold_right]?
+    Which is more common? *)
+Definition fold_right {A B}
+           (f : A -> B -> Comp B) (b : Comp B) (S : Ensemble A)
+: Comp B
+  := (ls <- to_list S;
+      List.fold_right (fun a b' => Bind b' (f a)) b ls).
+
+Definition Ensemble_fold_right {A B}
+           (f : A -> B -> B) (b : B) (S : Ensemble A)
+: Comp B
+  := fold_right (fun a b => ret (f a b)) (ret b) S.
+
+Lemma Ensemble_fold_right_simpl {A B} (f : A -> B -> B) b S
+: refineEquiv (@fold_right A B (fun a b' => ret (f a b')) (ret b) S)
+              (ls <- to_list S;
+               ret (List.fold_right f b ls)).
+Proof.
+  unfold fold_right.
+  f_equiv; intro ls; simpl.
+  induction ls; simpl; try reflexivity.
+  rewrite IHls.
+  autorewrite with refine_monad.
+  reflexivity.
+Qed.
+
+Lemma Ensemble_fold_right_simpl' {A B} f b S
+: refineEquiv (@Ensemble_fold_right A B f b S)
+              (ls <- to_list S;
+               ret (List.fold_right f b ls)).
+Proof.
+  exact (Ensemble_fold_right_simpl f b S).
+Qed.
