src/FiniteSetADTs/FiniteSetRefinement.v
@@ -1,0 +1,724 @@
+(** * Refinement of computations involving ensembles, to ones using finite sets *)
+Require Import Coq.Strings.String Coq.Sets.Ensembles Coq.Sets.Finite_sets Coq.Lists.List Coq.Sorting.Permutation.
+Require Import ADT ADT.ComputationalADT ADTRefinement.Core ADTNotation ADTRefinement.GeneralRefinements Common.AdditionalEnsembleDefinitions Common.AdditionalEnsembleLemmas Computation.
+Require Export FiniteSetADTs.FiniteSetADT.
+Require Import Common.
+
+(** TODO: Move this elsewhere *)
+Notation FullySharpenedComputation spec
+  := { c : _ | refine spec (ret c) }%type.
+
+(** We prove equivalences to handle various operations on ensembles,
+    and on lists equivalent to ensembles. *)
+Section FiniteSetHelpers.
+  Context (FiniteSetImpl : FullySharpened FiniteSetSpec).
+
+  Local Hint Extern 0 =>
+  match goal with
+    | [ H : False |- _ ] => destruct H
+    | [ H : false = true |- _ ] => solve [ inversion H ]
+    | [ H : true = false |- _ ] => solve [ inversion H ]
+  end.
+  Local Hint Extern 0 => apply Constructive_sets.Noone_in_empty.
+  Local Hint Resolve Constructive_sets.Add_intro2 Constructive_sets.Add_intro1.
+
+  Definition FiniteSetAndFunctionOfList {A} (f : W -> A -> A) (a : A)
+             (ls : list W)
+    := List.fold_right
+         (fun w xs_acc =>
+            let xs := fst xs_acc in
+            let acc := snd xs_acc in
+            ((if (snd (CallMethod (projT1 FiniteSetImpl) sIn xs w) : bool)
+             then xs
+             else fst (CallMethod (projT1 FiniteSetImpl) sAdd xs w)),
+             (if (snd (CallMethod (projT1 FiniteSetImpl) sIn xs w) : bool)
+              then acc
+              else f w acc)))
+         (CallConstructor (projT1 FiniteSetImpl) sEmpty tt,
+          a)
+         ls.
+
+  Definition FiniteSetAndListOfList (ls : list W)
+    := FiniteSetAndFunctionOfList (@cons _) nil ls.
+
+  Definition EnsembleOfList (ls : list W) : Ensemble W
+    := snd (FiniteSetAndFunctionOfList
+              (fun w xs => Ensembles.Add _ xs w)
+              (Ensembles.Empty_set _)
+              ls).
+
+  Definition FiniteSetOfList (ls : list W) : cRep (projT1 FiniteSetImpl)
+    := List.fold_right
+         (fun w xs =>
+            if (snd (CallMethod (projT1 FiniteSetImpl) sIn xs w) : bool)
+            then xs
+            else fst (CallMethod (projT1 FiniteSetImpl) sAdd xs w))
+         (CallConstructor (projT1 FiniteSetImpl) sEmpty tt)
+         ls.
+
+  Lemma NoFunctionJustFiniteSetOfFunction {A} f a ls
+  : fst (@FiniteSetAndFunctionOfList A f a ls) = FiniteSetOfList ls.
+  Proof.
+    unfold FiniteSetOfList.
+    unfold FiniteSetAndFunctionOfList.
+    simpl.
+    etransitivity; [ | eapply fst_fold_right ].
+    reflexivity.
+  Qed.
+
+  Definition NoListJustFiniteSetOfList ls
+  : fst (FiniteSetAndListOfList ls) = FiniteSetOfList ls
+    := NoFunctionJustFiniteSetOfFunction _ _ _.
+
+  Ltac handle_calls_then' tac :=
+    idtac;
+    let lem := match goal with
+                 | [ |- context[(CallMethod (projT1 ?impl) ?idx) ?rep ?arg] ]
+                   => constr:(fun rep' => ADTRefinementPreservesMethods (projT2 impl) {| bindex := idx |} rep' rep arg)
+                 | [ |- context[(CallConstructor (projT1 ?impl) ?idx) ?arg] ]
+                   => constr:(ADTRefinementPreservesConstructors (projT2 impl) {| bindex := idx |} arg)
+                 | [ H : context[(CallMethod (projT1 ?impl) ?idx) ?rep ?arg] |- _ ]
+                   => constr:(fun rep' => ADTRefinementPreservesMethods (projT2 impl) {| bindex := idx |} rep' rep arg)
+                 | [ H : context[(CallConstructor (projT1 ?impl) ?idx) ?arg] |- _ ]
+                   => constr:(ADTRefinementPreservesConstructors (projT2 impl) {| bindex := idx |} arg)
+               end in
+    let H' := fresh in
+    first [ pose proof (fun rep' H => lem rep' H _ (ReturnComputes _)) as H'
+          | pose proof (lem _ (ReturnComputes _)) as H' ];
+      simpl in H';
+      tac H'.
+
+  Local Ltac pre_t :=
+    repeat match goal with
+             | _ => progress inversion_by computes_to_inv
+             | _ => progress subst
+             | _ => progress simpl in *
+             | _ => progress split_iff
+             | _ => progress destruct_head bool
+             | [ H : ?x = ?x -> _ |- _ ] => specialize (H eq_refl)
+             | _ => assumption
+             | [ H : (_, _) = (_, _) |- _ ] => inversion H; clear H
+             | [ H : (_, _) = ?x |- _ ] => destruct x
+           end.
+
+  Lemma AbsR_EnsembleOfList_FiniteSetOfList ls
+  : AbsR (projT2 FiniteSetImpl) (EnsembleOfList ls) (FiniteSetOfList ls).
+  Proof.
+    induction ls; simpl;
+    handle_calls_then' ltac:(fun H => try specialize (H _ IHls));
+    pre_t;
+    unfold EnsembleOfList in *; simpl;
+    rewrite NoFunctionJustFiniteSetOfFunction;
+    handle_calls_then' ltac:(fun H => try specialize (H _ IHls));
+    pre_t.
+    { specialize_all_ways; auto. }
+    { specialize_all_ways; auto. }
+    { handle_calls_then' ltac:(fun H => try specialize (H _ IHls));
+      pre_t. }
+  Qed.
+
+  Lemma EnsembleOfList_In (ls : list W)
+  : forall x, Ensembles.In _ (EnsembleOfList ls) x <-> In x ls.
+  Proof.
+    induction ls;
+    repeat match goal with
+             | _ => split
+             | _ => progress split_iff
+             | [ H : Ensembles.In _ (Ensembles.Add _ _ _) _ |- _ ] => apply Constructive_sets.Add_inv in H
+             | [ H : Ensembles.In _ (Empty_set _) _ |- _ ] => apply Constructive_sets.Noone_in_empty in H
+             | _ => progress destruct_head or
+             | _ => progress destruct_head_hnf Empty_set
+             | _ => intro
+             | _ => progress subst
+             | _ => progress simpl in *
+             | _ => solve [ eauto ]
+             | _ => solve [ right; eauto ]
+             | _ => left; reflexivity
+             | _ => progress unfold EnsembleOfList in *
+             | [ H : context[if ?E then _ else _] |- _ ]
+               => revert H; case_eq E; intros
+             | [ |- context[if ?E then _ else _] ]
+               => case_eq E; intros
+             | [ H : _ |- _ ] => progress rewrite NoFunctionJustFiniteSetOfFunction in H
+           end.
+    handle_calls_then' ltac:(fun H => specialize (H _ (AbsR_EnsembleOfList_FiniteSetOfList _)));
+      pre_t.
+  Qed.
+
+  Local Ltac t :=
+    repeat match goal with
+             | _ => reflexivity
+             | _ => assumption
+             | _ => progress inversion_by computes_to_inv
+             | _ => progress subst
+             | _ => progress simpl in *
+             | _ => progress split_iff
+             | _ => progress destruct_head_hnf bool
+             | _ => split
+             | _ => intro
+             | [ H : ?T -> ?U, H' : ?T |- _ ] => specialize (H H')
+             | [ H : ?x = ?x -> _ |- _ ] => specialize (H eq_refl)
+             | [ H : (_, _) = (_, _) |- _ ] => inversion H; clear H
+             | [ H : (_, _) = ?x |- _ ] => destruct x
+           end.
+
+  Lemma classify_AbsR S fs
+  : AbsR (projT2 FiniteSetImpl) S fs
+    -> (forall x, Ensembles.In _ S x
+                   <-> snd (CallMethod (projT1 FiniteSetImpl) sIn fs x) = true).
+  Proof.
+    t.
+    { handle_calls_then' ltac:(fun H =>
+                                 match goal with
+                                   | [ H' : AbsR _ _ _ |- _ ] => specialize (H _ H')
+                                 end).
+      t. }
+    { handle_calls_then' ltac:(fun H =>
+                                 match goal with
+                                   | [ H' : AbsR _ _ _ |- _ ] => specialize (H _ H')
+                                 end).
+      t. }
+  Qed.
+
+  Local Hint Immediate EnsembleOfList_In AbsR_EnsembleOfList_FiniteSetOfList.
+
+  Lemma comp_split_snd {A B} (x : A * B)
+  : refineEquiv (ret (snd x))
+                (ab <- ret x;
+                 ret (snd ab)).
+  Proof.
+    autorewrite with refine_monad; reflexivity.
+  Qed.
+
+  Lemma refine_skip {A B C} (c : Comp A) (f : A -> Comp B) (dummy : A -> Comp C)
+  : refine (Bind c f)
+           (a <- c;
+            dummy a;;
+                  f a).
+  Proof.
+    repeat first [ intro
+                 | inversion_by computes_to_inv
+                 | econstructor; eassumption
+                 | econstructor; try eassumption; [] ].
+  Qed.
+
+  Lemma refine_skip2 {A B} (a : Comp A) (dummy : Comp B)
+  : refine a
+           (dummy;;
+            a).
+  Proof.
+    repeat first [ intro
+                 | inversion_by computes_to_inv
+                 | assumption
+                 | econstructor; eassumption
+                 | econstructor; try eassumption; [] ].
+  Qed.
+
+
+  Ltac handle_calls :=
+    repeat match goal with
+             | [ |- context[ret ((CallMethod (projT1 ?impl) ?idx) ?rep ?arg)] ]
+               => let lem := constr:(fun rep' => ADTRefinementPreservesMethods (projT2 impl) {| bindex := idx |} rep' rep arg) in
+                  simpl rewrite <- lem
+             | [ |- context[ret ((CallConstructor (projT1 ?impl) ?idx) ?arg)] ]
+               => let lem := constr:(ADTRefinementPreservesConstructors (projT2 impl) {| bindex := idx |} arg) in
+                  simpl rewrite <- lem
+           end.
+
+  Lemma finite_set_handle_cardinal_helper (ls : list W)
+  : refine (S <- { S : Ensemble W | forall x, Ensembles.In _ S x <-> List.In x ls  };
+            { n : nat | AdditionalEnsembleDefinitions.cardinal _ S n })
+           (ret (snd (CallMethod (projT1 FiniteSetImpl) sSize
+                                 (FiniteSetOfList ls)
+                                 tt))).
+  Proof.
+    etransitivity; [ | apply comp_split_snd ].
+    handle_calls; [ | apply AbsR_EnsembleOfList_FiniteSetOfList ].
+    repeat first [ progress simpl
+                 | rewrite <- refine_skip
+                 | autosetoid_rewrite with refine_monad ].
+    repeat intro; eauto.
+  Qed.
+
+  Lemma reverse_ensemble_list_equivalence_iff (S : Ensemble W)
+  : refineEquiv (ls <- {ls : list W | EnsembleListEquivalence S ls};
+                 {S0 : Ensemble W | forall x : W, Ensembles.In W S0 x <-> In x ls})
+                (ls <- {ls : list W | EnsembleListEquivalence S ls};
+                 { S' : _ | Same_set _ S' S }).
+  Proof.
+    split; repeat intro;
+    inversion_by computes_to_inv;
+    subst;
+    repeat constructor;
+    let x := match goal with H : EnsembleListEquivalence _ ?x |- _ => constr:x end in
+    apply BindComputes with (comp_a_value := x);
+      destruct_head_hnf and;
+      split_iff;
+      repeat constructor;
+      hnf;
+      auto.
+  Qed.
+
+  Lemma reverse_ensemble_list_equivalence_iff' {B} (S : Ensemble W) (f : _ -> Comp B)
+  : refineEquiv (ls <- {ls : list W | EnsembleListEquivalence S ls};
+                 Bind {S0 : Ensemble W | forall x : W, Ensembles.In W S0 x <-> In x ls} f)
+                (ls <- {ls : list W | EnsembleListEquivalence S ls};
+                 Bind { S' : _ | Same_set _ S' S } f).
+  Proof.
+    etransitivity; [ symmetry; apply refineEquiv_bind_bind | ].
+    rewrite reverse_ensemble_list_equivalence_iff.
+    apply refineEquiv_bind_bind.
+  Qed.
+
+  Lemma reverse_ensemble_list_equivalence_iff'' {B} (S : Ensemble W) (f : _ -> Comp B)
+  : refine (ls <- {ls : list W | EnsembleListEquivalence S ls};
+            Bind {S0 : Ensemble W | forall x : W, Ensembles.In W S0 x <-> In x ls} f)
+           ({ls : list W | EnsembleListEquivalence S ls};;
+            Bind { S' : _ | Same_set _ S' S } f).
+  Proof.
+    rewrite reverse_ensemble_list_equivalence_iff'.
+    reflexivity.
+  Qed.
+
+  (*Lemma reverse_ensemble_list_equivalence (S : Ensemble W)
+  : refineEquiv (ls <- {ls : list W | EnsembleListEquivalence S ls};
+                 ret (elements ls))
+                (ls <- {ls : list W | EnsembleListEquivalence S ls};
+                 { S' : _ | Same_set _ S' S }).
+  Proof.
+    split; repeat intro;
+    inversion_by computes_to_inv;
+    subst.
+    repeat constructor;
+    let x := match goal with H : EnsembleListEquivalence _ ?x |- _ => constr:x end in
+    apply BindComputes with (comp_a_value := x);
+      destruct_head_hnf and;
+      split_iff;
+      repeat constructor;
+      hnf;
+      auto.
+  Qed.
+
+  Lemma reverse_ensemble_list_equivalence' {B} (S : Ensemble W) (f : _ -> Comp B)
+  : refineEquiv (ls <- {ls : list W | EnsembleListEquivalence S ls};
+                 Bind {S0 : Ensemble W | forall x : W, Ensembles.In W S0 x <-> In x ls} f)
+                (ls <- {ls : list W | EnsembleListEquivalence S ls};
+                 Bind { S' : _ | Same_set _ S' S } f).
+  Proof.
+    etransitivity; [ symmetry; apply refineEquiv_bind_bind | ].
+    rewrite reverse_ensemble_list_equivalence.
+    apply refineEquiv_bind_bind.
+  Qed.
+
+  Lemma reverse_ensemble_list_equivalence'' {B} (S : Ensemble W) (f : _ -> Comp B)
+  : refine (ls <- {ls : list W | EnsembleListEquivalence S ls};
+            Bind {S0 : Ensemble W | forall x : W, Ensembles.In W S0 x <-> In x ls} f)
+           ({ls : list W | EnsembleListEquivalence S ls};;
+            Bind { S' : _ | Same_set _ S' S } f).
+  Proof.
+    rewrite reverse_ensemble_list_equivalence'.
+    reflexivity.
+  Qed.*)
+
+
+
+  Lemma finite_set_handle_cardinal (S : Ensemble W)
+  : refine { n : nat | AdditionalEnsembleDefinitions.cardinal _ S n }
+           (ls <- { ls : _ | EnsembleListEquivalence S ls };
+            ret (snd (CallMethod (projT1 FiniteSetImpl) sSize
+                                 (FiniteSetOfList ls)
+                                 tt))).
+  Proof.
+    simpl.
+    setoid_rewrite <- finite_set_handle_cardinal_helper.
+    rewrite reverse_ensemble_list_equivalence_iff'.
+    rewrite <- refine_skip2.
+    repeat intro;
+      inversion_by computes_to_inv;
+      constructor.
+    eapply cardinal_Same_set; eassumption.
+  Qed.
+
+  (*Lemma FiniteSetAndListOfList_spec1 ls S
+  : AbsR (projT2 FiniteSetImpl)
+         S
+         (fst (FiniteSetAndListOfList ls))
+    <-> EnsembleListEquivalence S (snd (FiniteSetAndListOfList ls)).
+  Proof.
+    revert S.
+    induction ls.
+    { simpl.
+      let lem := match goal with
+                   | [ |- context[CallConstructor (projT1 ?impl) ?idx ?arg] ]
+                     => constr:(ADTRefinementPreservesConstructors (projT2 impl) {| bindex := idx |} arg)
+                   | [ IHls : AbsR _ _ _ |- context[CallMethod (projT1 ?impl) ?idx ?rep ?arg] ]
+                     => constr:(ADTRefinementPreservesMethods (projT2 impl) {| bindex := idx |} _ rep arg IHls)
+                 end in
+      let lem' := constr:(lem  _ (ReturnComputes _)) in
+      pose proof lem';
+        inversion_by computes_to_inv;
+        subst.
+      intros; split.
+      { repeat (intro || split || constructor || simpl in * || auto).
+        match goal with
+          | [ x : W, H1 : AbsR _ _ _, H2 : AbsR _ _ _ |- _ ]
+            => let lem := constr:(ADTRefinementPreservesMethods
+                                    (projT2 FiniteSetImpl)
+                                    {| bindex := sIn |}) in
+               pose proof (lem _ _ x H1 _ (ReturnComputes _));
+                 pose proof (lem _ _ x H2 _ (ReturnComputes _))
+        end.
+        simpl in *.
+        inversion_by computes_to_inv.
+        repeat match goal with
+                 | _ => progress simpl in *
+                 | _ => progress subst
+                 | _ => progress split_iff
+                 | [ H : ?T -> ?U, H' : ?T |- _ ] => specialize (H H')
+                 | [ H : ?x = ?x -> _ |- _ ] => specialize (H eq_refl)
+                 | [ H : (_, _) = (_, _) |- _ ] => inversion H; clear H
+                 | [ H : (_, _) = ?x |- _ ] => destruct x
+                 | _ => progress destruct_head_hnf Empty_set
+               end. }
+      { repeat first [ intro
+                     | split
+                     | constructor
+                     | progress simpl in *
+                     | progress split_iff
+                     | progress destruct_head_hnf and ].
+        (** TODO: eliminate extensionality_ensembles here? *)
+        rewrite (Extensionality_Ensembles _ S (Empty_set _)); trivial.
+        split; hnf; intros; unfold Ensembles.In in *;
+        destruct_head_hnf Empty_set;
+        solve [ exfalso; eauto ]. } }
+    { simpl.
+      match goal with
+        | [ |- context[if ?E then _ else _] ] => case_eq E; intro
+      end; auto.
+      let lem := match goal with
+                   | [ H : appcontext[CallMethod (projT1 ?impl) ?idx ?rep ?arg] |- _ ]
+                     => constr:(fun rep' => ADTRefinementPreservesMethods (projT2 impl) {| bindex := idx |} rep' rep arg)
+                 end in
+      pose proof (fun rep' H => lem rep' H _ (ReturnComputes _));
+        simpl in *.
+      intro S.
+      specialize (H0 (Subtract _ S a)).
+      split.
+      { intro H'.
+
+      unfold refine in H0.
+      simpl in H0.
+      let lem' := constr:(lem  _ (ReturnComputes _)) in
+      pose proof lem';
+        inversion_by computes_to_inv;
+
+
+      edestruct cMethods.
+        exfalso; eauto.
+        unfold Same_set in *.
+        unfold Included in *.
+        unfold iff in *.
+ || auto).
+
+
+        hnf in H2, H3.
+        simpl in *.
+
+
+        assert (Ensembles.In _ (Empty_set _) x).
+        *)
+  Lemma AbsR_EnsembleOfList_FiniteSetOfListOfFiniteSetAndListOfList ls
+  : AbsR (projT2 FiniteSetImpl)
+         (EnsembleOfList ls)
+         (FiniteSetOfList (snd (FiniteSetAndListOfList ls))).
+  Proof.
+    induction ls; simpl.
+    { handle_calls_then' ltac:(fun H => idtac).
+      inversion_by computes_to_inv; subst; trivial. }
+    { handle_calls_then' ltac:(fun H =>
+                                 rewrite NoListJustFiniteSetOfList in *;
+                                 specialize (H _ (AbsR_EnsembleOfList_FiniteSetOfList _))).
+      inversion_by computes_to_inv.
+      destruct_head_hnf prod;
+      destruct_head_hnf bool;
+      t.
+      { unfold EnsembleOfList in *; simpl in *.
+        rewrite NoFunctionJustFiniteSetOfFunction in *.
+        handle_calls_then' ltac:(fun H =>
+                                   specialize (H _ (AbsR_EnsembleOfList_FiniteSetOfList _))).
+        t.
+        eauto. }
+      { unfold EnsembleOfList in *; simpl in *.
+        rewrite NoFunctionJustFiniteSetOfFunction in *.
+        let th :=
+            handle_calls_then' ltac:(fun H =>
+                                       match goal with
+                                         | [ H' : AbsR _ _ _ |- _ ]
+                                           => specialize (H _ H')
+                                         | _ => specialize (H _ (AbsR_EnsembleOfList_FiniteSetOfList _))
+                                       end) in
+        th;
+          inversion_by computes_to_inv;
+          t;
+          eauto;
+          th;
+          inversion_by computes_to_inv;
+          t;
+          eauto;
+          th;
+          inversion_by computes_to_inv;
+          t. } }
+  Qed.
+
+(*  Definition FiniteSetOfFiniteSetAndListOfList ls
+  : AbsR (projT2 FiniteSetImpl) (EnsembleOfList ls) (FiniteSetOfList (snd (FiniteSetAndListOfList ls))).
+  Proof.
+
+
+
+                (ret ).
+  Proof.*)
+
+  Lemma refine_EnsembleListEquivalenceAdd_iff {T} ls a
+  : refine (S <- {S : Ensemble T
+                 | forall x, Ensembles.In T S x <-> a = x \/ List.In x ls};
+            {ls' : list T | EnsembleListEquivalence S ls'})
+           (S <- {S : Ensemble T
+                 | forall x, Ensembles.In T S x <-> List.In x ls};
+            ls' <- {ls' : list T | EnsembleListEquivalence S ls'};
+            b <- { b : bool | b = true <-> List.In a ls };
+            ret (if b then ls' else a::ls')).
+  Proof.
+    repeat intro.
+    repeat match goal with
+             | [ H : computes_to (Bind _ _) _ |- _ ]
+               => apply computes_to_inv in H;
+                 destruct_head_hnf ex;
+                 destruct_head_hnf and
+             | [ H : computes_to (ret _) _ |- _ ]
+               => apply computes_to_inv in H
+             | _ => progress subst
+             | _ => progress inversion_by computes_to_inv
+             | _ => progress split_iff
+           end.
+    let S := match goal with H : Ensemble _ |- _ => constr:H end in
+    apply BindComputes with (comp_a_value := (Ensembles.Add _ S a));
+      constructor;
+      repeat match goal with
+               | _ => intro
+               | _ => split
+               | _ => progress destruct_head_hnf Union
+               | _ => progress destruct_head_hnf Singleton
+               | _ => progress destruct_head_hnf sumbool
+               | _ => progress destruct_head_hnf or
+               | _ => progress destruct_head_hnf and
+               | _ => progress destruct_head_hnf bool
+               | _ => progress split_iff
+               | _ => progress subst
+               | _ => solve [ left; eauto ]
+               | _ => solve [ right; eauto ]
+               | [ H : forall x, Ensembles.In _ _ _ -> _, H' : Ensembles.In _ _ _ |- _ ]
+                 => specialize (H _ H')
+               | _ => solve [ eauto ]
+               | _ => solve [ constructor; intuition ]
+             end.
+  Qed.
+
+  Local Hint Constructors NoDup.
+
+  Lemma refine_EnsembleListEquivalenceAdd {T} ls a
+  : refine {ls' : list T | EnsembleListEquivalence (elements (a::ls)) ls'}
+           (ls' <- {ls' : list T | EnsembleListEquivalence (elements ls) ls'};
+            b <- { b : bool | b = true <-> List.In a ls };
+            ret (if b then ls' else a::ls')).
+  Proof.
+    repeat intro.
+    repeat match goal with
+             | _ => assumption
+             | _ => right; assumption
+             | _ => intro
+             | [ H : computes_to (Bind _ _) _ |- _ ]
+               => apply computes_to_inv in H;
+                 destruct_head_hnf ex;
+                 destruct_head_hnf and
+             | [ H : computes_to (ret _) _ |- _ ]
+               => apply computes_to_inv in H
+             | [ H : ?x = ?x -> _ |- _ ] => specialize (H eq_refl)
+             | _ => progress subst
+             | _ => progress destruct_head_hnf bool
+             | _ => progress destruct_head_hnf or
+             | _ => progress inversion_by computes_to_inv
+             | _ => progress split_iff
+             | _ => apply PickComputes
+             | [ H : ?T -> false = true |- _ ]
+               => assert (~T)
+                 by (let H' := fresh in intro H'; specialize (H H'); inversion H);
+                 clear H
+             | [ |- EnsembleListEquivalence _ _ ] =>
+               eapply EnsembleListEquivalence_Same_set; try eassumption; []
+             | [ |- Same_set _ _ _ ] => split; repeat intro; hnf in *
+             | [ |- EnsembleListEquivalence _ _ ] => destruct_head_hnf and; split
+             | _ => progress unfold elements, Ensembles.In in *
+             | [ |- NoDup (_::_) ] => constructor
+             | _ => solve [ eauto ]
+             | [ |- _ <-> _ ] => split
+           end.
+  Qed.
+
+  Lemma finite_set_handle_EnsembleListEquivalence_iff (ls : list W)
+  : refine (S <- { S : Ensemble W | forall x, Ensembles.In _ S x <-> List.In x ls };
+            { ls' : _ | EnsembleListEquivalence S ls' })
+           (ret (snd (FiniteSetAndListOfList ls))).
+  Proof.
+    simpl.
+    induction ls; simpl.
+    { autosetoid_rewrite with refine_monad.
+      repeat first [ intro
+                   | progress simpl
+                   | rewrite <- refine_skip
+                   | progress autosetoid_rewrite with refine_monad
+                   | progress inversion_by computes_to_inv
+                   | progress subst ].
+      econstructor; repeat constructor; eauto; simpl; eauto. }
+    { rewrite refine_EnsembleListEquivalenceAdd_iff.
+      rewrite <- refineEquiv_bind_bind.
+      rewrite IHls; clear IHls.
+      autorewrite with refine_monad.
+      rewrite NoListJustFiniteSetOfList.
+      match goal with
+        | [ |- context[if ?E then _ else _] ] => case_eq E; intro
+      end;
+        handle_calls_then'
+          ltac:(fun H => specialize (H _ (AbsR_EnsembleOfList_FiniteSetOfList _)));
+        inversion_by computes_to_inv;
+        t.
+      { match goal with
+          | [ H : Ensembles.In _ (EnsembleOfList _) _ |- _ ] => apply EnsembleOfList_In in H
+        end.
+        apply BindComputes with (comp_a_value := true);
+        repeat constructor; eauto. }
+      { apply BindComputes with (comp_a_value := false);
+        repeat constructor; intros; eauto.
+        match goal with
+          | [ H : Ensembles.In _ (EnsembleOfList _) _ -> ?T |- ?T ]
+            => apply H, EnsembleOfList_In; trivial
+        end. } }
+  Qed.
+
+  Lemma finite_set_handle_EnsembleListEquivalence_iff' {A} (ls : list W) (f : _ -> Comp A)
+  : refine (S <- { S : Ensemble W | forall x, Ensembles.In _ S x <-> List.In x ls };
+            Bind { ls' : _ | EnsembleListEquivalence S ls' } f)
+           (f (snd (FiniteSetAndListOfList ls))).
+  Proof.
+    simpl.
+    rewrite <- refineEquiv_bind_bind.
+    rewrite finite_set_handle_EnsembleListEquivalence_iff; simpl.
+    match goal with
+      | [ |- context[ret ?x] ] => generalize x; intro
+    end.
+    autorewrite with refine_monad.
+    reflexivity.
+  Qed.
+
+  Lemma finite_set_handle_EnsembleListEquivalence (ls : list W)
+  : refine { ls' : _ | EnsembleListEquivalence (elements ls) ls' }
+           (ret (snd (FiniteSetAndListOfList ls))).
+  Proof.
+    simpl.
+    induction ls; simpl.
+    { autosetoid_rewrite with refine_monad.
+      repeat first [ intro
+                   | progress simpl
+                   | rewrite <- refine_skip
+                   | progress autosetoid_rewrite with refine_monad
+                   | progress inversion_by computes_to_inv
+                   | progress subst ].
+      econstructor; repeat constructor; eauto; simpl; eauto. }
+    { rewrite refine_EnsembleListEquivalenceAdd.
+      rewrite IHls; clear IHls.
+      autorewrite with refine_monad.
+      rewrite NoListJustFiniteSetOfList.
+      match goal with
+        | [ |- context[if ?E then _ else _] ] => case_eq E; intro
+      end;
+        handle_calls_then'
+          ltac:(fun H => specialize (H _ (AbsR_EnsembleOfList_FiniteSetOfList _)));
+        inversion_by computes_to_inv;
+        t.
+      { match goal with
+          | [ H : Ensembles.In _ (EnsembleOfList _) _ |- _ ] => apply EnsembleOfList_In in H
+        end.
+        apply BindComputes with (comp_a_value := true);
+        repeat constructor; eauto. }
+      { apply BindComputes with (comp_a_value := false);
+        repeat constructor; intros; eauto.
+        match goal with
+          | [ H : Ensembles.In _ (EnsembleOfList _) _ -> ?T |- ?T ]
+            => apply H, EnsembleOfList_In; trivial
+        end. } }
+  Qed.
+
+  Lemma CallSize_FiniteSetOfListOfFiniteSetAndListOfList ls arg
+  : snd
+      ((CallMethod (projT1 FiniteSetImpl) sSize)
+         (FiniteSetOfList (snd (FiniteSetAndListOfList ls)))
+         arg)
+    = snd ((CallMethod (projT1 FiniteSetImpl) sSize)
+             (FiniteSetOfList ls)
+             arg).
+  Proof.
+    do 2 (handle_calls_then' ltac:(fun H =>
+                                     first [ specialize (H _ (AbsR_EnsembleOfList_FiniteSetOfListOfFiniteSetAndListOfList _))
+                                           | specialize (H _ (AbsR_EnsembleOfList_FiniteSetOfList _)) ]);
+          inversion_by computes_to_inv;
+          t).
+    eapply cardinal_unique; eassumption.
+  Qed.
+
+  Lemma fold_right_snd_FiniteSetAndListOfList {A} (f : W -> A -> A) (a : A) ls
+  : List.fold_right f a (snd (FiniteSetAndListOfList ls))
+    = snd (FiniteSetAndFunctionOfList f a ls).
+  Proof.
+    simpl.
+    induction ls; simpl; trivial.
+    unfold FiniteSetAndListOfList in *.
+    rewrite <- IHls.
+    rewrite !NoFunctionJustFiniteSetOfFunction.
+    match goal with
+      | [ |- context[if ?x then _ else _] ] => case_eq x; intro
+    end;
+      reflexivity.
+  Qed.
+End FiniteSetHelpers.
+
+Create HintDb finite_sets discriminated.
+
+Hint Unfold FiniteSetADT.to_list FiniteSetADT.cardinal FiniteSetADT.fold_right : finite_sets.
+
+Ltac start_FullySharpenedComputation :=
+  eexists;
+  match goal with
+    | [ |- refine ?a ?b ] => let a' := eval hnf in a in change (refine a' b)
+  end.
+
+Ltac finish_FullySharpenedComputation :=
+  reflexivity.
+
+Notation Sharpening x := (refine x (ret _)).
+
+Tactic Notation "begin" "sharpening" "computation" := start_FullySharpenedComputation.
+
+Tactic Notation "finish" "sharpening" "computation" := finish_FullySharpenedComputation.
+
+Ltac finite_set_sharpen_step FiniteSetImpl :=
+  first [ setoid_rewrite (@finite_set_handle_cardinal FiniteSetImpl)
+        | rewrite (@finite_set_handle_EnsembleListEquivalence FiniteSetImpl)
+        | rewrite (@CallSize_FiniteSetOfListOfFiniteSetAndListOfList FiniteSetImpl)
+        | rewrite (@fold_right_snd_FiniteSetAndListOfList FiniteSetImpl)
+        | rewrite Ensemble_fold_right_simpl
+        | rewrite Ensemble_fold_right_simpl'
+        | progress autounfold with finite_sets
+        | progress autorewrite with refine_monad ].
+
+Tactic Notation "sharpen" "computation" "with" "FiniteSet" "implementation" ":=" constr(FiniteSetImpl) :=
+  repeat finite_set_sharpen_step FiniteSetImpl.
